Remove Arith_ext and beq_nat
Signed-off-by: Nicolas Iooss <nicolas.iooss_git@polytechnique.org>

substitution.v
@@ -1,4 +1,57 @@
-Require Import Arith_ext free_variables lterm.
+Require Import Arith free_variables lterm.
+
+(** Substitute a variable, (Var n)[x <- u], d = Var n before recursion *)
+Fixpoint subst_var (n x: nat) (u d: lterm) : lterm :=
+  match n, x with
+    | O, O => u
+    | O, S _ => d
+    | S _, O => d
+    | S m, S y => subst_var m y u d
+  end
+.
+
+Lemma subst_var_eq:
+  forall (n: nat) (u d: lterm), subst_var n n u d = u.
+Proof.
+  induction n; intros u d; simpl; trivial.
+Save.
+
+Lemma subst_var_lt_diff:
+  forall (y n: nat) (u d: lterm), subst_var n (n + S y) u d = d.
+Proof.
+  induction y; induction n; intros u d; simpl; trivial.
+Save.
+
+Lemma subst_var_lt:
+  forall (n x: nat) (u d: lterm), n < x -> subst_var n x u d = d.
+Proof.
+  intros n x u d H.
+  cut (x = n + S (pred (x - n))).
+    intro Hx. rewrite Hx. apply subst_var_lt_diff.
+  elim (S_pred (x - n) O). auto with arith.
+  apply (plus_lt_reg_l O (x - n) n).
+  rewrite (plus_comm n O).
+  rewrite <- (le_plus_minus n x); auto with arith.
+Save.
+
+Lemma subst_var_gt_diff:
+  forall (y n: nat) (u d: lterm), subst_var (n + S y) n u d = d.
+Proof.
+  induction y; induction n; intros u d; simpl; trivial.
+Save.
+
+Lemma subst_var_gt:
+  forall (n x: nat) (u d: lterm), n > x -> subst_var n x u d = d.
+Proof.
+  intros n x u d H.
+  cut (n = x + S (pred (n - x))).
+    intro Hx. rewrite Hx. apply subst_var_gt_diff.
+  elim (S_pred (n - x) O). auto with arith.
+  apply (plus_lt_reg_l O (n - x) x).
+  rewrite (plus_comm x O).
+  rewrite <- (le_plus_minus x n); auto with arith.
+Save.
+
 
 (**
  * Substitute x with u in t, ie. return t[x <- u]
@@ -9,7 +62,7 @@ Require Import Arith_ext free_variables lterm.
  *)
 Fixpoint subst (t: lterm) (x: nat) (u: lterm) : lterm :=
   match t with
-    | Var y => if beq_nat x y then u else t
+    | Var n => subst_var n x u (Var n)
     | Lambda t0 => Lambda (subst t0 (S x) u)
     | Apply t0 u0 => Apply (subst t0 x u) (subst u0 x u)
   end
@@ -20,16 +73,11 @@ Lemma substitute_freevar_eq:
   forall (t: lterm) (x: nat) (u: lterm), fr_below x t -> subst t x u = t.
 Proof.
   induction t; simpl; intros x u H.
-    assert (beq_nat x n = false).
-      rewrite (beq_nat_false_iff x n).
-      apply lt_neq_sym; trivial.
-    rewrite H0; trivial.
-
+    apply subst_var_lt; trivial.
     rewrite (IHt (S x) u); trivial.
-
     destruct H.
-    rewrite (IHt1 x u); trivial.
-    rewrite (IHt2 x u); trivial.
+      rewrite (IHt1 x u); trivial.
+      rewrite (IHt2 x u); trivial.
 Save.
 
 (** Substitution on a closed term does nothing *)
