Makefile
@@ -31,8 +31,8 @@ beta_reduction.vo: lterm.vo substitution.vo
 compiler_correct.vo: beta_reduction.vo compiler.vo free_variables.vo krivine.vo
 compiler_correct.vo: lterm.vo substitute_list.vo substitute_varlist.vo
 compiler.vo: free_variables.vo krivine.vo lterm.vo substitute_list.vo
-free_variables.vo: Arith_ext.vo lterm.vo
+free_variables.vo: lterm.vo
 identity.vo: beta_reduction.vo compiler.vo compiler_correct.vo free_variables.vo krivine.vo lterm.vo
-substitute_list.vo: Arith_ext.vo free_variables.vo lterm.vo substitution.vo substitute_varlist.vo
-substitute_varlist.vo: Arith_ext.vo lterm.vo substitution.vo
-substitution.vo: Arith_ext.vo free_variables.vo lterm.vo
+substitute_list.vo: free_variables.vo lterm.vo substitution.vo substitute_varlist.vo
+substitute_varlist.vo: lterm.vo substitution.vo
+substitution.vo: free_variables.vo lterm.vo
